Iterator/SimpleIterator.lean
@@ -35,7 +35,7 @@ instance (m) [Monad m] : MonadLift (CodensityT m) (IterationT m) where
 def IterationT.liftWithProperty {p : γ → Prop} (t : CodensityT m { c : γ // p c }) : IterationT m γ :=
   { property := p, computation := t }
 
-@[inline]
+@[always_inline, inline]
 def IterationT.mapH {γ : Type u} {m : Type w → Type w'} [Monad m]
     {δ : Type v}
     (f : γ → δ)
@@ -43,12 +43,13 @@ def IterationT.mapH {γ : Type u} {m : Type w → Type w'} [Monad m]
   { property d := ∃ c, d = f c ∧ t.property c,
     computation := t.computation.mapH fun c => ⟨f c.1, c.1, rfl, c.2⟩ }
 
-@[inline]
+@[always_inline, inline]
 def IterationT.bindH {m : Type w → Type w'} [Monad m] {γ : Type u} {δ : Type v}
     (t : IterationT m γ) (f : γ → IterationT m δ) : IterationT m δ :=
   { property d := ∃ c, (f c).property d ∧ t.property c
     computation := t.computation.bindH fun c => (f c.1).computation.mapH fun d => ⟨d.1, c.1, d.2, c.2⟩}
 
+@[always_inline, inline]
 def IterationT.liftInnerMonad {γ : Type w} {m : Type w → Type w'} [Pure m] (n : Type w → Type w'') [Monad n] [MonadLift m n] (t : IterationT m γ) :
     IterationT n γ :=
   { property := t.property
@@ -58,27 +59,16 @@ variable {α : Type u} {m : Type w → Type w'} {β : Type v}
 
 variable (m) in
 @[always_inline, inline]
-def IterationT.step [Iterator α m β] [Monad m] (it : α) : IterationT m (IterStep.for m it) :=
-  { property
-      | .yield it' b _ => Iterator.yielded m it it' b
-      | .skip it' _ => Iterator.skipped m it it'
-      | .done _ => Iterator.done m it,
-    computation := (fun step => ⟨step, match step with
-        | .yield _ _ h => h
-        | .skip _ h => h
-        | .done h => h⟩) <$> Iterator.step it }
+def IterationT.step [Iterator α m β] [Monad m] (it : α) : IterationT m (IterStep α β) :=
+  { property := Iterator.plausible_step m it
+    computation := Iterator.step it }
 
 class SimpleIterator (α : Type u) (m : Type w → Type w') (β : outParam (Type v)) where
-  step : α → IterationT m (RawStep α β)
+  step : α → IterationT m (IterStep α β)
 
 instance [SimpleIterator α m β] [Monad m] : Iterator α m β where
-  yielded it it' output := SimpleIterator.step (m := m) it |>.property <| .yield it' output ⟨⟩
-  skipped it it' := SimpleIterator.step it (m := m) |>.property <| .skip it' ⟨⟩
-  done it := SimpleIterator.step (m := m) it |>.property <| .done ⟨⟩
-  step it := (match · with
-    | ⟨.yield it' output _, h⟩ => .yield it' output h
-    | ⟨.skip it' _, h⟩ => .skip it' h
-    | ⟨.done _, h⟩ => .done h) <$> (SimpleIterator.step (α := α) (m := m) it).computation
+  plausible_step it := SimpleIterator.step it |>.property
+  step it := (SimpleIterator.step (α := α) (m := m) it).computation
 
 variable (α m) in
 class SimpleIterator.Finite [SimpleIterator α m β] [Monad m] where
@@ -90,7 +80,7 @@ variable (α m) in
 class SimpleIterator.Productive [SimpleIterator α m β] [Monad m] where
   rel : α → α → Prop
   wf : WellFounded rel
-  subrelation : {it it' : α} → (SimpleIterator.step (m := m) it).property (.skip it' ⟨⟩) → rel it' it
+  subrelation : {it it' : α} → (SimpleIterator.step (m := m) it).property (.skip it') → rel it' it
 
 instance [SimpleIterator α m β] [Monad m] [SimpleIterator.Finite α m] : Finite α m where
   wf := by
@@ -98,8 +88,8 @@ instance [SimpleIterator α m β] [Monad m] [SimpleIterator.Finite α m] : Finit
     · intro x y h
       apply SimpleIterator.Finite.subrelation
       obtain ⟨b, h⟩ | h := h
-      · exact ⟨.yield x.inner b ⟨⟩, rfl, h⟩
-      · exact ⟨.skip x.inner ⟨⟩, rfl, h⟩
+      · exact ⟨.yield x.inner b, rfl, h⟩
+      · exact ⟨.skip x.inner, rfl, h⟩
     · apply InvImage.wf
       exact SimpleIterator.Finite.wf
 
@@ -119,9 +109,9 @@ def matchStepH {α : Type u} {β : Type v} {m : Type w → Type w'} [Monad m]
     (it : α)
     (yield : α → β → IterationT m γ) (skip : α → IterationT m γ) (done : IterationT m γ) : IterationT m γ :=
   IterationT.step m it |>.bindH (match · with
-  | .yield it' b _ => yield it' b
-  | .skip it' _ => skip it'
-  | .done _ => done)
+  | .yield it' b => yield it' b
+  | .skip it' => skip it'
+  | .done => done)
 
 @[always_inline, inline]
 def matchStep {γ : Type max u v} [Monad m]
@@ -130,17 +120,17 @@ def matchStep {γ : Type max u v} [Monad m]
   matchStepH it yield skip done
 
 theorem successor_yield [Monad m] [Pure m] [SimpleIterator α m β] {it₁ it₂ : α} {b : β} :
-    ((pure (IterStep.yield it₁ b True.intro) : IterationT m (RawStep α β)).mapH IterStep.successor).property (some it₂) ↔
+    ((pure (.yield it₁ b) : IterationT m (IterStep α β)).mapH IterStep.successor).property (some it₂) ↔
       it₂ = it₁ := by
   simp [IterationT.mapH, Pure.pure, IterStep.successor]
 
 theorem successor_skip [Monad m] [Pure m] [SimpleIterator α m β] {it₁ it₂ : α} :
-    ((pure (IterStep.skip it₁ ⟨⟩) : IterationT m (RawStep α β)).mapH IterStep.successor).property (some it₂) ↔
+    ((pure (.skip it₁) : IterationT m (IterStep α β)).mapH IterStep.successor).property (some it₂) ↔
       it₂ = it₁ := by
   simp [IterationT.mapH, Pure.pure, IterStep.successor]
 
 theorem successor_done [Monad m] [Pure m] [SimpleIterator α m β] {it: α} :
-    ((pure (IterStep.done True.intro) : IterationT m (RawStep α β)).mapH IterStep.successor).property (some it) ↔ False := by
+    ((pure .done : IterationT m (IterStep α β)).mapH IterStep.successor).property (some it) ↔ False := by
   simp [IterationT.mapH, Pure.pure, IterStep.successor]
 
 theorem successor_matchStepH {α : Type u} {m : Type w → Type w'} {β : Type v} {γ : Type x} {δ : Type y}
@@ -148,9 +138,9 @@ theorem successor_matchStepH {α : Type u} {m : Type w → Type w'} {β : Type v
     {it : α} {yield skip done}
     {f : γ → δ} {x : δ}
     (h : (IterationT.mapH f <| matchStepH (m := m) (γ := γ) it yield skip done).property x) :
-    (∃ it' b, Iterator.yielded m it it' b ∧ (IterationT.mapH f <| yield it' b).property x) ∨
-    (∃ it', Iterator.skipped m it it' ∧ (IterationT.mapH f <| skip it').property x) ∨
-    (Iterator.done m it ∧ (IterationT.mapH f done).property x) := by
+    (∃ it' b, Iterator.plausible_step m it (.yield it' b) ∧ (IterationT.mapH f <| yield it' b).property x) ∨
+    (∃ it', Iterator.plausible_step m it (.skip it') ∧ (IterationT.mapH f <| skip it').property x) ∨
+    (Iterator.plausible_step m it .done ∧ (IterationT.mapH f done).property x) := by
   simp only [IterationT.mapH, IterationT.bindH, matchStepH] at h
   obtain ⟨c, rfl, _, h, h'⟩ := h
   split at h
@@ -162,9 +152,9 @@ theorem successor_matchStep {α : Type u} {m : Type w → Type w'} {β : Type v}
     [Monad m] [Iterator α m β] {it : α} {yield skip done}
     {f : γ → δ} {x : δ}
     (h : (IterationT.mapH f <| matchStep (m := m) (γ := γ) it yield skip done).property x) :
-    (∃ it' b, Iterator.yielded m it it' b ∧ (IterationT.mapH f <| yield it' b).property x) ∨
-    (∃ it', Iterator.skipped m it it' ∧ (IterationT.mapH f <| skip it').property x) ∨
-    (Iterator.done m it ∧ (IterationT.mapH f done).property x) :=
+    (∃ it' b, Iterator.plausible_step m it (.yield it' b) ∧ (IterationT.mapH f <| yield it' b).property x) ∨
+    (∃ it', Iterator.plausible_step m it (.skip it')  ∧ (IterationT.mapH f <| skip it').property x) ∨
+    (Iterator.plausible_step m it .done ∧ (IterationT.mapH f done).property x) :=
   successor_matchStepH h
 
 theorem property_matchStepH {α : Type u} {m : Type w → Type w'} {β : Type v} {γ : Type x}
@@ -172,9 +162,9 @@ theorem property_matchStepH {α : Type u} {m : Type w → Type w'} {β : Type v}
     {it : α} {yield skip done}
     {x : γ}
     (h : (matchStepH (m := m) (γ := γ) it yield skip done).property x) :
-    (∃ it' b, Iterator.yielded m it it' b ∧ (yield it' b).property x) ∨
-    (∃ it', Iterator.skipped m it it' ∧ (skip it').property x) ∨
-    (Iterator.done m it ∧ done.property x) := by
+    (∃ it' b, Iterator.plausible_step m it (.yield it' b) ∧ (yield it' b).property x) ∨
+    (∃ it', Iterator.plausible_step m it (.skip it') ∧ (skip it').property x) ∨
+    (Iterator.plausible_step m it .done ∧ done.property x) := by
   simp only [IterationT.bindH, matchStepH] at h
   obtain ⟨c, h, h'⟩ := h
   split at h
@@ -187,9 +177,9 @@ theorem computation_matchStepH {α : Type u} {m : Type w → Type w'} {β : Type
     {it : α} {yield skip done} :
     (matchStepH (m := m) (γ := γ) it yield skip done).computation =
       (IterationT.step m it).computation.bindH (match · with
-        | ⟨.yield it' out h, h'⟩ => (yield it' out).computation.mapH (fun y => ⟨y.1, .yield it' out h, y.2, h'⟩)
-        | ⟨.skip it' h, h'⟩ => (skip it').computation.mapH (fun y => ⟨y.1, .skip it' h, y.2, h'⟩)
-        | ⟨.done h, h'⟩ => done.computation.mapH (fun y => ⟨y.1, .done h, y.2, h'⟩)) := by
+        | ⟨.yield it' out, h'⟩ => (yield it' out).computation.mapH (fun y => ⟨y.1, .yield it' out, y.2, h'⟩)
+        | ⟨.skip it', h'⟩ => (skip it').computation.mapH (fun y => ⟨y.1, .skip it', y.2, h'⟩)
+        | ⟨.done, h'⟩ => done.computation.mapH (fun y => ⟨y.1, .done, y.2, h'⟩)) := by
   simp only [matchStepH, IterationT.bindH]
   refine congrArg (fun x => (IterationT.step m it).computation.bindH x) ?_
   ext x; cases x
