Iterator/IterationT.lean
@@ -1,0 +1,56 @@
+/-
+Copyright (c) 2025 Lean FRO, LLC. All rights reserved.
+Released under Apache 2.0 license as described in the file LICENSE.
+Authors: Paul Reichert
+-/
+prelude
+import Init.Core
+import Init.Ext
+import Iterator.Cont
+
+@[ext]
+structure IterationT (m : Type w → Type w') (γ : Type u) where
+  property : γ → Prop
+  computation : CodensityT m { c : γ // property c }
+
+instance : Monad (IterationT m) where
+  pure a := { property b := (b = a)
+              computation := pure ⟨a, rfl⟩ }
+  bind x f := { property a := ∃ b, (f b).property a ∧ x.property b
+                computation := do
+                  let b ← x.computation
+                  let a ← (f b).computation
+                  return ⟨a.1, b.1, a.2, b.2⟩ }
+
+theorem IterationT.computation_pure {m : Type w → Type w'} {γ : Type u} {a : γ} :
+    (pure a : IterationT m γ).computation = pure ⟨a, rfl⟩ := rfl
+
+instance (m) [Monad m] : MonadLift m (IterationT m) where
+  monadLift t := { property := fun _ => True, computation := (⟨·, True.intro⟩) <$> t }
+
+instance (m) [Monad m] : MonadLift (CodensityT m) (IterationT m) where
+  monadLift t := { property := fun _ => True, computation := (⟨·, True.intro⟩) <$> t }
+
+@[always_inline, inline]
+def IterationT.liftWithProperty {p : γ → Prop} (t : CodensityT m { c : γ // p c }) : IterationT m γ :=
+  { property := p, computation := t }
+
+@[always_inline, inline]
+def IterationT.mapH {γ : Type u} {m : Type w → Type w'} [Monad m]
+    {δ : Type v}
+    (f : γ → δ)
+    (t : IterationT m γ) : IterationT m δ :=
+  { property d := ∃ c, d = f c ∧ t.property c,
+    computation := t.computation.mapH fun c => ⟨f c.1, c.1, rfl, c.2⟩ }
+
+@[always_inline, inline]
+def IterationT.bindH {m : Type w → Type w'} [Monad m] {γ : Type u} {δ : Type v}
+    (t : IterationT m γ) (f : γ → IterationT m δ) : IterationT m δ :=
+  { property d := ∃ c, (f c).property d ∧ t.property c
+    computation := t.computation.bindH fun c => (f c.1).computation.mapH fun d => ⟨d.1, c.1, d.2, c.2⟩}
+
+@[always_inline, inline]
+def IterationT.liftInnerMonad {γ : Type w} {m : Type w → Type w'} [Pure m] (n : Type w → Type w'') [Monad n] [MonadLift m n] (t : IterationT m γ) :
+    IterationT n γ :=
+  { property := t.property
+    computation := monadLift t.computation.run }
