Iterator/Producers.lean
@@ -16,9 +16,10 @@ structure ListIterator (α : Type u) where
   list : List α
 
 instance {α} : Iterator (ListIterator α) m α where
-  yielded it it' a := it.list = a :: it'.list
-  skipped _ _ := False
-  done it := it.list = []
+  plausible_step it
+    | .yield it' a => it.list = a :: it'.list
+    | .skip _ => False
+    | .done => it.list = []
   step
     | { list := .nil } => pure <| .done rfl
     | { list := x :: xs } => pure <| .yield { list := xs } x rfl
@@ -42,7 +43,7 @@ theorem ListIterator.subrelation :
       (InvImage WellFoundedRelation.rel (ListIterator.list ∘ FiniteIteratorWF.inner)) := by
   intro x y hlt
   simp_wf
-  simp only [FiniteIteratorWF.lt, Iterator.yielded, Iterator.skipped, or_false] at hlt
+  simp only [FiniteIteratorWF.lt, Iterator.plausible_step, or_false] at hlt
   cases hlt
   simp_all
 
@@ -61,9 +62,10 @@ structure UnfoldIterator (α : Type u) (f : α → α) where
   next : α
 
 instance : Iterator (UnfoldIterator α f) m α where
-  yielded it it' a := it.next = a ∧ it'.next = f a
-  skipped _ _ := False
-  done _ := False
+  plausible_step it
+    | .yield it' a => it.next = a ∧ it'.next = f a
+    | .skip _ => False
+    | .done => False
   step
     | ⟨a⟩ => pure <| .yield ⟨f a⟩ a ⟨rfl, rfl⟩
 
